SimAsm.thy
@@ -2,14 +2,72 @@ theory SimAsm
   imports Soundness
 begin
 
+section \<open>State\<close>
+
 datatype ('g,'r) var = Reg 'r | Glb 'g
-type_synonym ('v,'g,'r) state = "('g,'r) var \<Rightarrow> 'v"
+record ('v,'a) state_rec = st :: "'a \<Rightarrow> 'v"
+
+type_synonym ('v,'g,'r,'a) state = "('v,('g,'r) var,'a) state_rec_scheme"
+type_synonym ('v,'g,'a) gstate = "('v,'g,'a) state_rec_scheme"
+
+type_synonym ('v,'g,'r,'a) pred = "('v,'g,'r,'a) state set"
+type_synonym ('v,'g,'a) gpred = "('v,'g,'a) gstate set"
+
+type_synonym ('v,'g,'r,'a) trel = "('v,'g,'r,'a) state rel"
+type_synonym ('v,'g,'a) grel = "('v,'g,'a) gstate rel"
+
+type_synonym ('v,'g,'r,'a) trans = "('v,'g,'r,'a) pred \<Rightarrow> ('v,'g,'r,'a) pred"
+type_synonym ('v,'g,'r,'a) rtrans = "('v,'g,'r,'a) trel \<Rightarrow> ('v,'g,'r,'a) trel"
+
+type_synonym ('v,'g,'r,'a) auxfn = "('v,('g,'r) var,'a) state_rec_scheme \<Rightarrow> 'a"
+
+definition glb
+  where "glb m \<equiv> \<lambda>v. m (Glb v)"
+
+definition rg
+  where "rg m \<equiv> \<lambda>v. m (Reg v)"
+
+section \<open>Write Operations\<close>
+
+definition st_upd :: "('v,'a,'b) state_rec_scheme \<Rightarrow> 'a \<Rightarrow> 'v \<Rightarrow> ('v,'a,'b) state_rec_scheme"
+  where "st_upd m a b = m \<lparr> st := ((st m) (a := b)) \<rparr>"
+
+definition aux_upd :: "('v,'r,'a) state_rec_scheme \<Rightarrow> (('v,'r,'a) state_rec_scheme \<Rightarrow> 'a) \<Rightarrow> ('v,'r,'a) state_rec_scheme"
+  where "aux_upd m f \<equiv> m\<lparr>state_rec.more := f m\<rparr>"
+
+nonterminal updbinds and updbind
+
+syntax
+  "_updbindm" :: "'a \<Rightarrow> 'a \<Rightarrow> updbind"            ("(2_ :=\<^sub>s/ _)")
+  "_updbinda" :: "'a \<Rightarrow> updbind"                  ("(2aux:/ _)")
+  ""         :: "updbind \<Rightarrow> updbinds"             ("_")
+  "_updbinds":: "updbind \<Rightarrow> updbinds \<Rightarrow> updbinds" ("_,/ _")
+  "_Update"  :: "'a \<Rightarrow> updbinds \<Rightarrow> 'a"            ("_/'((_)')" [1000, 0] 900)
+
+translations
+  "_Update f (_updbinds b bs)" \<rightleftharpoons> "_Update (_Update f b) bs"
+  "f(x:=\<^sub>sy)" \<rightleftharpoons> "CONST st_upd f x y"
+  "f(aux: y)" \<rightleftharpoons> "CONST aux_upd f y"
+
+lemma [simp]:
+  "st (m(r :=\<^sub>s e)) q = (if r = q then e else st m q)"
+  by (auto simp: st_upd_def)
+
+lemma aux_nop [simp]:
+  "m(aux:more) = m"
+  by (auto simp: aux_upd_def)
+
+lemma st_upd_twist: "a \<noteq> c \<Longrightarrow> (m(a :=\<^sub>s b))(c :=\<^sub>s d) = (m(c :=\<^sub>s d))(a :=\<^sub>s b)"
+  unfolding st_upd_def by (auto intro!: equality fun_upd_twist)
+
+section \<open>Expression Language\<close>
+
 datatype ('v,'g,'r) exp = Var "('g,'r) var" | Val 'v | Exp "'v list \<Rightarrow> 'v" "('v,'g,'r) exp list"
 
 text \<open>Evaluate an expression given a state\<close>
-fun ev :: "('v,'g,'r) state \<Rightarrow> ('v,'g,'r) exp \<Rightarrow> 'v"
+fun ev :: "('v,'g,'r,'a) state \<Rightarrow> ('v,'g,'r) exp \<Rightarrow> 'v"
   where 
-    "ev m (Var r) = m r" |
+    "ev m (Var r) = st m r" |
     "ev _ (Val v) = v" |
     "ev m (Exp f rs) = f (map (ev m) rs)"
 
@@ -30,7 +88,7 @@ fun subst :: "('v,'g,'r) exp \<Rightarrow> ('g,'r) var \<Rightarrow> ('v,'g,'r) 
 datatype ('v,'g,'r) bexp = Neg "('v,'g,'r) bexp" | Exp\<^sub>B "'v list \<Rightarrow> bool" "('v,'g,'r) exp list"
 
 text \<open>Evaluate an expression given a state\<close>
-fun ev\<^sub>B :: "('v,'g,'r) state \<Rightarrow> ('v,'g,'r) bexp \<Rightarrow> bool"
+fun ev\<^sub>B :: "('v,'g,'r,'a) state \<Rightarrow> ('v,'g,'r) bexp \<Rightarrow> bool"
   where 
     "ev\<^sub>B m (Neg e) = (\<not> (ev\<^sub>B m e))" |
     "ev\<^sub>B m (Exp\<^sub>B f rs) = f (map (ev m) rs)"
@@ -47,48 +105,88 @@ fun subst\<^sub>B :: "('v,'g,'r) bexp \<Rightarrow> ('g,'r) var \<Rightarrow> ('
     "subst\<^sub>B (Neg b) r e = Neg (subst\<^sub>B b r e)" |
     "subst\<^sub>B (Exp\<^sub>B f rs) r e = (Exp\<^sub>B f (map (\<lambda>x. subst x r e) rs))"
 
+lemma [simp]:
+  "ev m (subst e r f) = ev (m(r :=\<^sub>s (ev m f))) e"
+proof (induct e)
+  case (Exp fn rs)
+  hence [simp]: "map (ev m \<circ> (\<lambda>x. subst x r f)) rs = map (ev (m(r :=\<^sub>s ev m f))) rs"
+    by auto
+  show ?case by simp
+qed auto
+
+lemma ev_nop [simp]:
+  "r \<notin> deps e \<Longrightarrow> ev (m(r :=\<^sub>s f)) e = ev m e"
+proof (induct e)
+  case (Exp fn rs)
+  hence [simp]: "map (ev (m(r :=\<^sub>s f))) rs = map (ev m) rs" by auto
+  show ?case by simp
+qed auto
+
+lemma [simp]:
+  "ev\<^sub>B m (subst\<^sub>B b r e) = ev\<^sub>B (m(r :=\<^sub>s (ev m e))) b"
+proof (induct b)
+  case (Exp\<^sub>B fn rs)
+  have [simp]: "map (ev m \<circ> (\<lambda>x. subst x r e)) rs = map (ev (m(r :=\<^sub>s ev m e))) rs"
+    by (auto simp: fun_upd_def)     
+  show ?case by simp
+qed simp
+
+lemma ev\<^sub>B_nop [simp]:
+  "r \<notin> deps\<^sub>B b \<Longrightarrow> ev\<^sub>B (m(r :=\<^sub>s f)) b = ev\<^sub>B m b"
+proof (induct b)
+  case (Exp\<^sub>B fn rs)
+  hence [simp]: "map (ev (m(r :=\<^sub>s f))) rs = map (ev m) rs"
+    using ev_nop[of r _ m f] by (auto simp: fun_upd_def) 
+  show ?case by simp
+qed simp
+
 section \<open>Operations\<close>
 
 datatype ('v,'g,'r) op =
     assign "('g,'r) var" "('v,'g,'r) exp"
   | cmp "('v,'g,'r) bexp"
-  | fence
-  | cfence
+  | full_fence
+  | ctrl_fence
   | nop
 
-fun beh\<^sub>i :: "('v,'g,'r) op \<Rightarrow> ('v,'g,'r) state rel"
+abbreviation ncmp
+  where "ncmp b \<equiv> cmp (Neg b)"
+
+fun beh\<^sub>i :: "('v,'g,'r) op \<Rightarrow> ('v,'g,'r,'a) state rel"
   where
-    "beh\<^sub>i (assign a e) = {(m,m'). m' = m (a := ev m e)}" |
+    "beh\<^sub>i (assign a e) = {(m,m'). m' = m (a :=\<^sub>s ev m e)}" |
     "beh\<^sub>i (cmp b) = {(m,m'). m = m' \<and> ev\<^sub>B m b}" |
     "beh\<^sub>i _ = Id"
 
-text \<open>Variables written by a sub-operation\<close>
+text \<open>Variables written by an operation\<close>
 fun wr :: "('v,'g,'r) op \<Rightarrow> ('g,'r) var set"
   where 
     "wr (assign y _) = {y}" |
     "wr _ = {}"
 
-text \<open>Variables read by a sub-operation\<close>
+text \<open>Variables read by an operation\<close>
 fun rd :: "('v,'g,'r) op \<Rightarrow> ('g,'r) var set"
   where
     "rd (assign _ e) = deps e" |
     "rd (cmp b) = deps\<^sub>B b" |
     "rd _ = {}"
 
+text \<open>Variables referenced by an operation\<close>
 abbreviation refs
   where "refs a \<equiv> wr a \<union> rd a"
 
+text \<open>Domain of register variables\<close>
 abbreviation locals
   where "locals \<equiv> Reg ` UNIV"
 
-text \<open>Sub-Instruction Reordering\<close>
+text \<open>Instruction Reordering\<close>
 text \<open>Only pattern match on first argument due to performance issues\<close>
 fun re\<^sub>i :: "('v,'g,'r) op \<Rightarrow> ('v,'g,'r) op \<Rightarrow> bool" 
   where
-    "re\<^sub>i fence \<alpha> = False" |
-    "re\<^sub>i (cmp b) \<alpha> = (wr \<alpha> \<subseteq> locals \<and> \<alpha> \<noteq> cfence \<and> rd (cmp b) \<inter> wr \<alpha> = {} \<and> rd (cmp b) \<inter> rd \<alpha> \<subseteq> locals)" |
-    "re\<^sub>i cfence \<alpha> = (rd \<alpha> \<subseteq> locals)" |
-    "re\<^sub>i \<alpha> \<beta> = (\<alpha> \<noteq> fence \<and> wr \<alpha> \<inter> wr \<beta> = {} \<and> rd \<alpha> \<inter> wr \<beta> = {} \<and> refs \<alpha> \<inter> refs \<beta> \<subseteq> locals)"
+    "re\<^sub>i full_fence \<alpha> = False" |
+    "re\<^sub>i (cmp b) \<alpha> = (\<alpha> \<noteq> full_fence \<and> \<alpha> \<noteq> ctrl_fence \<and> wr \<alpha> \<subseteq> locals \<and> rd (cmp b) \<inter> wr \<alpha> = {} \<and> rd (cmp b) \<inter> rd \<alpha> \<subseteq> locals)" |
+    "re\<^sub>i ctrl_fence \<alpha> = (\<alpha> \<noteq> full_fence \<and> rd \<alpha> \<subseteq> locals)" |
+    "re\<^sub>i \<alpha> \<beta> = (\<beta> \<noteq> full_fence \<and> wr \<alpha> \<inter> wr \<beta> = {} \<and> rd \<alpha> \<inter> wr \<beta> = {} \<and> refs \<alpha> \<inter> refs \<beta> \<subseteq> locals)"
 
 text \<open>Sub-Instruction Forwarding\<close>
 fun fwd\<^sub>i :: "('v,'g,'r) op \<Rightarrow> ('v,'g,'r) op \<Rightarrow> ('v,'g,'r) op" 
@@ -100,60 +198,59 @@ fun fwd\<^sub>i :: "('v,'g,'r) op \<Rightarrow> ('v,'g,'r) op \<Rightarrow> ('v,
 definition comp (infix "\<Otimes>" 60)
   where "comp a b \<equiv> {(m,m'). \<exists>m''. (m,m'') \<in> a \<and> (m'',m') \<in> b}"
 
-lemma [simp]:
-  "ev m (subst e r f) = ev (m(r := (ev m f))) e"
-proof (induct e)
-  case (Exp fn rs)
-  hence [simp]: "map (ev m \<circ> (\<lambda>x. subst x r f)) rs = map (ev (\<lambda>a. if a = r then ev m f else m a)) rs"
-    by auto
-  show ?case by simp
-qed auto
-
-lemma ev_nop [simp]:
-  "r \<notin> deps e \<Longrightarrow> ev (m(r := f)) e = ev m e"
-proof (induct e)
-  case (Exp fn rs)
-  hence [simp]: "map (ev (\<lambda>a. if a = r then f else m a)) rs = (map (ev m) rs)" by auto
-  show ?case by simp
-qed auto
-
-lemma [simp]:
-  "ev\<^sub>B m (subst\<^sub>B b r e) = ev\<^sub>B (m(r := (ev m e))) b"
-proof (induct b)
-  case (Exp\<^sub>B fn rs)
-  have [simp]: "map (ev m \<circ> (\<lambda>x. subst x r e)) rs = map (ev (\<lambda>a. if a = r then ev m e else m a)) rs"
-    by (auto simp: fun_upd_def)     
-  show ?case by simp
-qed simp
-
-lemma ev\<^sub>B_nop [simp]:
-  "r \<notin> deps\<^sub>B b \<Longrightarrow> ev\<^sub>B (m(r := f)) b = ev\<^sub>B m b"
-proof (induct b)
-  case (Exp\<^sub>B fn rs)
-  hence [simp]: "map (ev (\<lambda>a. if a = r then f else m a)) rs = map (ev m) rs"
-    using ev_nop[of r _ m f] by (auto simp: fun_upd_def) 
-  show ?case by simp
-qed simp
-
 lemma re_consistent:
-  "re\<^sub>i \<alpha> (fwd\<^sub>i \<beta> \<alpha>) \<Longrightarrow> beh\<^sub>i \<alpha> \<Otimes> beh\<^sub>i \<beta> \<supseteq> beh\<^sub>i (fwd\<^sub>i \<beta> \<alpha>) \<Otimes> beh\<^sub>i \<alpha>" 
-  by (cases \<alpha>; cases \<beta>; auto simp add: comp_def)
+  "re\<^sub>i \<alpha> (fwd\<^sub>i \<beta> \<alpha>) \<Longrightarrow> beh\<^sub>i \<alpha> \<Otimes> beh\<^sub>i \<beta> \<supseteq> beh\<^sub>i (fwd\<^sub>i \<beta> \<alpha>) \<Otimes> beh\<^sub>i \<alpha>"
+  by (cases \<alpha>; cases \<beta>, auto simp: comp_def intro!: st_upd_twist)
 
-type_synonym ('v,'g,'r) opbasic = "(('v,'g,'r) op, ('v,'g,'r) state) basic"
+section \<open>Auxiliary State Updates\<close>
+
+text \<open>
+We wish to support auxiliary state to support more abstract reasoning about data structures
+and concurrency.
+This is achieved by allowing arbitrary extensions to the state representation, which
+can be updated atomically at any sub-operation.
+This auxiliary state cannot influence real execution behaviour by definition.
+\<close>
+type_synonym ('v,'g,'r,'a) auxop = "('v,'g,'r) op \<times> ('v,'g,'r,'a) auxfn"
+
+fun beh\<^sub>a :: "('v,'g,'r,'a) auxop \<Rightarrow> ('v,'g,'r,'a) state rel"
+  where "beh\<^sub>a (\<alpha>,f) = beh\<^sub>i \<alpha> O {(m,m'). m' = m(aux: f)}"
+
+fun re\<^sub>a :: "('v,'g,'r,'a) auxop \<Rightarrow> ('v,'g,'r,'a) auxop \<Rightarrow> bool" 
+  where "re\<^sub>a (\<alpha>,f) (\<beta>,f') = re\<^sub>i \<alpha> \<beta>"
+
+fun fwd\<^sub>a :: "('v,'g,'r,'a) auxop \<Rightarrow> ('v,'g,'r,'a) auxop \<Rightarrow> ('v,'g,'r,'a) auxop" 
+  where "fwd\<^sub>a (\<alpha>,f) (\<beta>,f') = (fwd\<^sub>i \<alpha> \<beta>,f)"
+
+section \<open>Instruction Specification Language\<close>
+
+text \<open>
+To instantiate the abstract theory, we must couple each sub-operation with its precondition
+and behaviour in a tuple\<close>
+type_synonym ('v,'g,'r,'a) opbasic = "(('v,'g,'r,'a) auxop, ('v,'g,'r,'a) state) basic"
  
 text \<open>Duplicate forwarding and reordering behaviour of underlying instruction\<close>
-fun fwd\<^sub>s :: "('v,'g,'r) opbasic \<Rightarrow> ('v,'g,'r) op \<Rightarrow> ('v,'g,'r) opbasic" 
-  where "fwd\<^sub>s (\<alpha>,v,_) \<beta> =  (fwd\<^sub>i \<alpha> \<beta>, v, beh\<^sub>i (fwd\<^sub>i \<alpha> \<beta>))" 
+fun fwd\<^sub>s :: "('v,'g,'r,'a) opbasic \<Rightarrow> ('v,'g,'r,'a) auxop \<Rightarrow> ('v,'g,'r,'a) opbasic" 
+  where "fwd\<^sub>s (\<alpha>,v,_) \<beta> =  (fwd\<^sub>a \<alpha> \<beta>, v, beh\<^sub>a (fwd\<^sub>a \<alpha> \<beta>))" 
+
+text \<open>Lift an operation with specification\<close>
+definition liftg :: "('v,'g,'r,'a) pred \<Rightarrow> ('v,'g,'r) op \<Rightarrow> ('v,'g,'r,'a) auxfn \<Rightarrow> ('v,'g,'r,'a) opbasic" 
+  ("\<lfloor>_,_,_\<rfloor>" 100)
+  where "liftg v \<alpha> f \<equiv> ((\<alpha>,f), v, beh\<^sub>a (\<alpha>,f))"
+
+text \<open>Lift an operation without specification\<close>
+definition liftl :: "('v,'g,'r) op \<Rightarrow> ('v,'g,'r,'a) opbasic" 
+  ("\<lfloor>_\<rfloor>" 100)
+  where "liftl \<alpha> \<equiv> ((\<alpha>,state_rec.more), UNIV, beh\<^sub>a (\<alpha>,state_rec.more))"
 
 section \<open>Language Definition\<close>
 
-datatype ('v,'g,'r) lang =
+datatype ('v,'g,'r,'a) lang =
   Skip
-  | Op "('v,'g,'r) state set" "('v,'g,'r) op"
-  | Seq "('v,'g,'r) lang" "('v,'g,'r) lang"
-  | If "('v,'g,'r) bexp" "('v,'g,'r) lang" "('v,'g,'r) lang"
-  | While "('v,'g,'r) bexp" "('v,'g,'r) state set" "('v,'g,'r) lang"
-
-interpretation rules fwd\<^sub>s re\<^sub>i by (unfold_locales) (auto)
+  | Op "('v,'g,'r,'a) pred" "('v,'g,'r) op" "('v,'g,'r,'a) auxfn"
+  | Seq "('v,'g,'r,'a) lang" "('v,'g,'r,'a) lang"
+  | If "('v,'g,'r) bexp" "('v,'g,'r,'a) lang" "('v,'g,'r,'a) lang"
+  | While "('v,'g,'r) bexp" "('v,'g,'r,'a) pred" "('v,'g,'r,'a) lang"
+  | DoWhile "('v,'g,'r,'a) pred" "('v,'g,'r,'a) lang" "('v,'g,'r) bexp"
 
 end
