SimAsm_Rules.thy
@@ -5,24 +5,10 @@ begin
 section \<open>Wellformedness\<close>
 
 definition glb
-  where "glb m \<equiv> \<lambda>v. m (Glb v)"
+  where "glb m \<equiv> \<lparr> st = (\<lambda>v. st m (Glb v)), \<dots> = more m \<rparr>"
 
 definition rg
-  where "rg m \<equiv> \<lambda>v. m (Reg v)"
-
-type_synonym ('v,'g) gstate = "'g \<Rightarrow> 'v"
-type_synonym ('v,'g) grel = "('v,'g) gstate rel"
-type_synonym ('v,'g,'r) trel = "('v,'g,'r) state rel"
-type_synonym ('v,'g,'r) trans = "('v,'g,'r) state set \<Rightarrow> ('v,'g,'r) state set"
-type_synonym ('v,'r,'a) rtrans = "('v,'r,'a) trel \<Rightarrow> ('v,'r,'a) trel"
-
-text \<open>Lift a relational predicate and assume it preserves the thread state\<close>
-definition step\<^sub>t :: "('v,'g) grel \<Rightarrow> ('v,'g,'r) trel"
-  where "step\<^sub>t R \<equiv> {(m,m'). (glb m, glb m') \<in> R \<and> rg m = rg m'}"
-
-text \<open>Define stability in terms of a relational predicate that preserves the thread state\<close>
-abbreviation stable\<^sub>t
-  where "stable\<^sub>t R P \<equiv> stable (step\<^sub>t R) P"
+  where "rg m \<equiv> \<lambda>v. st m (Reg v)"
 
 definition stabilize
   where "stabilize R P \<equiv> {m. \<forall>m'. (glb m,glb m') \<in> R \<longrightarrow> rg m = rg m' \<longrightarrow> m' \<in> P}"
@@ -33,8 +19,23 @@ definition reflexive
 definition transitive
   where "transitive R \<equiv> \<forall>m m' m''. (m,m') \<in> R \<longrightarrow> (m',m'') \<in> R \<longrightarrow> (m,m'') \<in> R"
 
+definition assert
+  where "assert b \<equiv> {m. b}"
+
+text \<open>Lift a relational predicate and assume it preserves the thread state\<close>
+definition step\<^sub>t :: "('v,'g,'a) grel \<Rightarrow> ('v,'g,'r,'a) trel"
+  where "step\<^sub>t R \<equiv> {(m,m'). (glb m, glb m') \<in> R \<and> rg m = rg m'}"
+
+text \<open>Lift a relational predicate\<close>
+definition step :: "('v,'g,'a) grel \<Rightarrow> ('v,'g,'r,'a) trel"
+  where "step R \<equiv> {(m,m'). (glb m, glb m') \<in> R}"
+
+text \<open>Define stability in terms of a relational predicate that preserves the thread state\<close>
+abbreviation stable\<^sub>t
+  where "stable\<^sub>t R P \<equiv> stable (step\<^sub>t R) P"
+
 text \<open>Couple all wellformedness conditions into a single definition\<close>
-abbreviation wellformed :: "('v,'a) grel \<Rightarrow> ('v,'a) grel \<Rightarrow> bool"
+abbreviation wellformed :: "('v,'g,'a) grel \<Rightarrow> ('v,'g,'a) grel \<Rightarrow> bool"
   where "wellformed R G \<equiv> reflexive R \<and> transitive R \<and> reflexive G" 
 
 text \<open>Show that a stabilized predicate is stable\<close>
@@ -68,40 +69,41 @@ proof -
 qed
 
 text \<open>Stabilization preserves entailment\<close>
-lemma stabilize_entail [intro!]:
+lemma stabilize_entail :
+  assumes "m \<in> stabilize R P" 
   assumes "reflexive R"
   assumes "P \<subseteq> Q"
-  shows "stabilize R P \<subseteq> Q"
-  using assms by (auto elim: stabilizeE)
+  shows "m \<in> stabilize R Q"
+  using assms by (auto simp: stabilize_def)
 
 section \<open>Predicate Transformations\<close>
 
-named_theorems wp_defs
-
 text \<open>Transform a predicate based on an sub-operation\<close>
-fun wp\<^sub>i :: "('v,'g,'r) op \<Rightarrow> ('v,'g,'r) trans" 
+fun wp\<^sub>i :: "('v,'g,'r) op \<Rightarrow> ('v,'g,'r,'a) trans" 
   where 
-    "wp\<^sub>i (assign r e) Q = {m. (m (r := ev m e)) \<in> Q}" |
+    "wp\<^sub>i (assign r e) Q = {m. (m (r :=\<^sub>s ev m e)) \<in> Q}" |
     "wp\<^sub>i (cmp b) Q =  {m. ev\<^sub>B m b \<longrightarrow> m \<in> Q}" | 
     "wp\<^sub>i _ Q = Q"
 
-definition assert
-  where "assert b \<equiv> {m. b}"
+text \<open>Transform a predicate based on an auxiliary state update\<close>
+fun wp\<^sub>a :: "('v,'g,'r,'a) auxfn \<Rightarrow> ('v,'g,'r,'a) trans"
+  where "wp\<^sub>a a Q = {m. m(aux: a) \<in> Q}"
 
 text \<open>Transform a predicate based on a program c within an environment R\<close>
-fun wp :: "('v,'g) grel \<Rightarrow> ('v,'g,'r) lang \<Rightarrow> ('v,'g,'r) trans"
+fun wp :: "('v,'g,'a) grel \<Rightarrow> ('v,'g,'r,'a) lang \<Rightarrow> ('v,'g,'r,'a) trans"
   where
     "wp R Skip Q = Q" |
-    "wp R (Op v a) Q = stabilize R (v \<inter> wp\<^sub>i a Q)" |
+    "wp R (Op v a f) Q = stabilize R (v \<inter> wp\<^sub>i a (wp\<^sub>a f Q))" |
     "wp R (Seq c\<^sub>1 c\<^sub>2) Q = wp R c\<^sub>1 (wp R c\<^sub>2 Q)" |
-    "wp R (If b c\<^sub>1 c\<^sub>2) Q = (wp\<^sub>i (cmp b) (wp R c\<^sub>1 Q) \<inter> wp\<^sub>i (cmp (Neg b)) (wp R c\<^sub>2 Q))" |
+    "wp R (If b c\<^sub>1 c\<^sub>2) Q = stabilize R (wp\<^sub>i (cmp b) (wp R c\<^sub>1 Q) \<inter> wp\<^sub>i (ncmp b) (wp R c\<^sub>2 Q))" |
     "wp R (While b I c) Q = 
-      (stabilize R I \<inter> assert (I \<subseteq> wp\<^sub>i (cmp b) (wp R c (stabilize R I)) \<inter> wp\<^sub>i (cmp (Neg b)) Q))"
+      (stabilize R I \<inter> assert (I \<subseteq> wp\<^sub>i (cmp b) (wp R c (stabilize R I)) \<inter> wp\<^sub>i (ncmp b) Q))" |
+    "wp R (DoWhile I c b) Q = 
+      (stabilize R I \<inter> assert (I \<subseteq> wp R c (stabilize R (wp\<^sub>i (cmp b) (stabilize R I) \<inter> wp\<^sub>i (ncmp b) Q))))"
 
 text \<open>Convert a predicate transformer into a relational predicate transformer\<close>
-definition wp\<^sub>r :: "('v,'r,'a) trans \<Rightarrow> ('v,'r,'a) rtrans"
+definition wp\<^sub>r :: "('v,'g,'r,'a) trans \<Rightarrow> ('v,'g,'r,'a) rtrans"
   where "wp\<^sub>r f G \<equiv> {(m,m'). m' \<in> f {m'. (m,m') \<in> G}}"
-declare wp\<^sub>r_def [wp_defs]
 
 subsection \<open>Guarantee Checks\<close>
 
@@ -112,18 +114,226 @@ abbreviation guar
 text \<open>Ensure all global operations in a thread conform to its guarantee\<close>
 fun guar\<^sub>c
   where 
-    "guar\<^sub>c (Op v a) G = (v \<subseteq> guar (wp\<^sub>i a) G)" |
+    "guar\<^sub>c Skip G = True" |
+    "guar\<^sub>c (Op v a f) G = (v \<subseteq> guar (wp\<^sub>i a o wp\<^sub>a f) (step G))" |
     "guar\<^sub>c (Seq c\<^sub>1 c\<^sub>2) G = (guar\<^sub>c c\<^sub>1 G \<and> guar\<^sub>c c\<^sub>2 G)" |
     "guar\<^sub>c (If _ c\<^sub>1 c\<^sub>2) G = (guar\<^sub>c c\<^sub>1 G \<and> guar\<^sub>c c\<^sub>2 G)" |
     "guar\<^sub>c (While _ _ c) G = (guar\<^sub>c c G)" |
-    "guar\<^sub>c _ _ = False"
+    "guar\<^sub>c (DoWhile _ c _) G = (guar\<^sub>c c G)"
+
+section \<open>Locale Interpretation\<close>
+
+text \<open>Convert the language into the abstract language expected by the underlying logic\<close> 
+fun lift\<^sub>c :: "('v,'g,'r,'a) lang \<Rightarrow> (('v,'g,'r,'a) auxop, ('v,'g,'r,'a) state) com"
+  where
+    "lift\<^sub>c Skip = com.Nil" |
+    "lift\<^sub>c (Op v a f) = Basic (\<lfloor>v,a,f\<rfloor>)" |
+    "lift\<^sub>c (lang.Seq c\<^sub>1 c\<^sub>2) = (com.Seq (lift\<^sub>c c\<^sub>1) (lift\<^sub>c c\<^sub>2))" |
+    "lift\<^sub>c (If b c\<^sub>1 c\<^sub>2) = (Choice 
+      (com.Seq (Basic (\<lfloor>cmp b\<rfloor>)) (lift\<^sub>c c\<^sub>1)) (com.Seq (Basic (\<lfloor>ncmp b\<rfloor>)) (lift\<^sub>c c\<^sub>2)))" |
+    "lift\<^sub>c (While b I c) = (com.Seq ((com.Seq (Basic (\<lfloor>cmp b\<rfloor>)) (lift\<^sub>c c))*) (Basic (\<lfloor>ncmp b\<rfloor>)))" | 
+    "lift\<^sub>c (DoWhile I c b) = (lift\<^sub>c c ;; Basic (\<lfloor>cmp b\<rfloor>))* ;; lift\<^sub>c c ;; Basic (\<lfloor>ncmp b\<rfloor>)" 
+
+text \<open>The language is always thread-local\<close>
+lemma local_lift [intro]:
+  "local (lift\<^sub>c c)"
+  by (induct c) auto
 
 text \<open>Correctness of the guarantee check\<close>
 lemma com_guar:
-  "wellformed R G \<Longrightarrow> guar\<^sub>c c G \<Longrightarrow> \<forall>\<beta>\<in>basics c. guar\<^sub>\<alpha> \<beta> G"
-proof (induct c)
-  case (Basic x)
-  then show ?case apply (cases "tag x") apply (auto simp: guar_def wp\<^sub>r_def) sorry
-qed auto
+  "wellformed R G \<Longrightarrow> guar\<^sub>c c G \<Longrightarrow> \<forall>\<beta>\<in>basics (lift\<^sub>c c). guar\<^sub>\<alpha> \<beta> (step G)"
+proof (induct c) 
+  case (Op v p)
+  then show ?case by (cases p) (auto simp: liftg_def guar_def wp\<^sub>r_def)
+qed (auto simp: guar_def reflexive_def liftl_def step_def)
+
+interpretation rules fwd\<^sub>s re\<^sub>a by (unfold_locales) (auto)
+
+abbreviation rules_abv ("_,_ \<turnstile> _ {_} _" [20,0,0,0,20] 20)
+  where "rules_abv \<equiv> rules"
+
+abbreviation lifted_abv ("_,_ \<turnstile>\<^sub>s _ {_} _" [20,0,0,0,20] 20)
+  where "lifted_abv R G P c Q \<equiv> step\<^sub>t R,step G \<turnstile> P {lift\<^sub>c c} Q"
+
+abbreviation validity_abv  ("\<Turnstile> _ SAT [_, _, _, _]" [60,0,0,0] 45) 
+  where "validity_abv c P R G Q \<equiv> validity (lift\<^sub>c c) P (step\<^sub>t R) (step G) Q"
+
+text \<open>An ordering property on contexts\<close>
+definition context_order 
+  ("_,_ \<turnstile>\<^sub>w _ \<ge> _" [100,0,0,100] 60)
+  where "context_order R G P Q \<equiv> 
+    (stable\<^sub>t R Q \<and> wellformed R G) \<longrightarrow> ((P \<subseteq> Q) \<and> stable\<^sub>t R P)"
+
+text \<open>The validity property we intend to show, abstracts over the preservation of wellformedness\<close>
+definition valid 
+  ("_,_ \<turnstile>\<^sub>w _ {_} _" [100,0,0,0,100] 60)
+  where "valid R G P c Q \<equiv>  
+    (wellformed R G \<and> stable\<^sub>t R Q \<and> guar\<^sub>c c G) \<longrightarrow> (stable\<^sub>t R P \<and> (R,G \<turnstile>\<^sub>s P {c} Q))"
+
+section \<open>Soundness\<close>
+
+text \<open>Basic Rule for operations with vc\<close>
+lemma basic_wp\<^sub>i_1:
+  assumes "P \<subseteq> stabilize R (c \<inter> wp\<^sub>i \<alpha> (wp\<^sub>a f Q))" "wellformed R G" "stable\<^sub>t R Q" 
+  assumes "c \<subseteq> guar (wp\<^sub>i \<alpha> o wp\<^sub>a f) (step G)"
+  shows "step\<^sub>t R,step G \<turnstile> P {Basic (\<lfloor>c, \<alpha>, f\<rfloor>)} Q"
+proof -
+  have "step\<^sub>t R,step G \<turnstile>\<^sub>A stabilize R (c \<inter> wp\<^sub>i \<alpha> (wp\<^sub>a f Q)) {\<lfloor>c, \<alpha>, f\<rfloor>} Q"
+    using assms by (cases \<alpha>) (auto simp: atomic_rule_def guar_def wp_def step_def 
+                                         wp\<^sub>r_def o_def liftg_def elim!: stabilizeE)
+  thus ?thesis using assms by (intro conseq[OF basic]) (auto)
+qed
+
+text \<open>Basic Rule for operations\<close>
+lemma basic_wp\<^sub>i_2:
+  assumes "P \<subseteq> stabilize R (wp\<^sub>i \<alpha> Q)" "wellformed R G" "stable\<^sub>t R Q"
+  assumes "\<forall>m. m \<in> guar (wp\<^sub>i \<alpha>) (step G)"
+  shows "step\<^sub>t R,step G \<turnstile> P {Basic (\<lfloor>\<alpha>\<rfloor>)} Q"
+proof -
+  have "step\<^sub>t R,step G \<turnstile>\<^sub>A stabilize R (wp\<^sub>i \<alpha> Q) {\<lfloor>\<alpha>\<rfloor>} Q"
+    using assms by (cases \<alpha>) (auto simp: atomic_rule_def guar_def wp_def step_def 
+                                         wp\<^sub>r_def o_def liftl_def elim!: stabilizeE)
+  thus ?thesis using assms by (intro conseq[OF basic]) (auto simp:)
+qed
+
+text \<open>A rule for cmp operations, used for If/While\<close>
+lemma cmp_sound [intro!]:
+  assumes "wellformed R G" "stable\<^sub>t R Q"
+  assumes "P \<subseteq> stabilize R (wp\<^sub>i (cmp b) Q)"
+  shows "step\<^sub>t R,step G \<turnstile> P {Basic (\<lfloor>cmp b\<rfloor>)} Q"
+  using assms by (intro basic_wp\<^sub>i_2) (auto simp: step_def reflexive_def wp\<^sub>r_def)
+
+subsection \<open>State Ordering\<close>
+
+text \<open>Properties of the state ordering. Essentially entailment with preservation of stability\<close>
+
+text \<open>The ordering is reflexive\<close>
+lemma refl_ord:
+  "R,G \<turnstile>\<^sub>w P \<ge> P"
+  unfolding context_order_def by (auto simp: )
+
+text \<open>It is possible to strengthen the RHS\<close>
+lemma assert_ord:
+  "R,G \<turnstile>\<^sub>w P \<inter> assert A \<ge> P"
+  by (cases A) (auto simp: context_order_def assert_def) 
+
+text \<open>Stabilize Ordering\<close>
+lemma stabilize_ord [intro]:
+  assumes "P \<subseteq> Q" 
+  shows "R,G \<turnstile>\<^sub>w stabilize R P \<ge> Q"
+  using assms stabilizeE unfolding context_order_def 
+  by blast
+
+subsection \<open>Rules\<close>
+
+text \<open>If Rule\<close>
+lemma if_wp:
+  "R,G \<turnstile>\<^sub>w P\<^sub>1 {c\<^sub>1} Q \<Longrightarrow> R,G \<turnstile>\<^sub>w P\<^sub>2 {c\<^sub>2} Q \<Longrightarrow> R,G \<turnstile>\<^sub>w stabilize R (wp\<^sub>i (cmp b) P\<^sub>1 \<inter> wp\<^sub>i (ncmp b) P\<^sub>2) {If b c\<^sub>1 c\<^sub>2} Q"
+  unfolding valid_def apply clarsimp apply (intro conjI rules.choice rules.seq, auto )
+  apply (rule stabilize_entail, auto)+
+  done
+
+text \<open>While Rule\<close>
+lemma while_wp:
+  assumes "R,G \<turnstile>\<^sub>w P {c} stabilize R J" (is "R,G \<turnstile>\<^sub>w P {c} ?I")
+  assumes "J \<subseteq>  (wp\<^sub>i (cmp b) P \<inter> wp\<^sub>i (ncmp b) Q)"
+  shows "R,G \<turnstile>\<^sub>w ?I {While b J c} Q"
+  unfolding valid_def lift\<^sub>c.simps
+proof (intro impI conjI rules.choice rules.seq)
+  assume "wellformed R G \<and> stable\<^sub>t R Q \<and> guar\<^sub>c (While b J c) (G)"
+  thus "step\<^sub>t R,step G \<turnstile> ?I {(Basic (\<lfloor>cmp b\<rfloor>) ;; lift\<^sub>c c)*} ?I"
+    using assms 
+    apply (intro rules.loop rules.seq, unfold valid_def)
+    apply force
+    apply force
+    apply (auto simp:)
+    apply (rule stabilize_entail, auto)+
+    done
+qed (insert assms, auto, rule stabilize_entail)
+
+text \<open>Do While Rule\<close>
+lemma do_wp:
+  assumes "R,G \<turnstile>\<^sub>w stabilize R J {c} stabilize R (wp\<^sub>i (cmp b) (stabilize R J) \<inter> (wp\<^sub>i (ncmp b) Q))" (is "R,G \<turnstile>\<^sub>w ?I {c} ?Q")
+  shows "R,G \<turnstile>\<^sub>w stabilize R J {DoWhile J c b} Q"
+  unfolding valid_def lift\<^sub>c.simps
+proof (intro impI conjI rules.choice rules.seq)
+  assume "wellformed R G \<and> stable\<^sub>t R Q \<and> guar\<^sub>c (DoWhile J c b) (G)"
+  thus "step\<^sub>t R,step G \<turnstile> ?I {lift\<^sub>c c} ?Q" 
+    using assms by (auto simp: valid_def) 
+next
+  assume "wellformed R G \<and> stable\<^sub>t R Q \<and> guar\<^sub>c (DoWhile J c b) (G)"
+  thus "step\<^sub>t R,step G \<turnstile> ?I {(lift\<^sub>c c ;; Basic (\<lfloor>cmp b\<rfloor>))*} ?I"
+    using assms 
+    apply (intro rules.loop rules.seq)
+    defer 1
+    apply auto[1]
+    apply (auto)[1]
+    apply (auto)
+    unfolding valid_def
+    by (simp add: rules.intros(8) stabilize_entail stabilize_stable subsetI)
+qed (insert assms, auto, rule stabilize_entail, auto)
+
+text \<open>False Rule\<close>
+lemma false_wp:
+  assumes "P = {}"
+  shows "R,G \<turnstile>\<^sub>w P {c} Q"
+  using assms unfolding valid_def
+  by (intro conjI impI com_guar rules.conseq[OF falseI, where ?G="step G"]) (auto)
+
+text \<open>Rewrite Rule\<close>
+lemma rewrite_wp:
+  "R,G \<turnstile>\<^sub>w P {c} Q \<Longrightarrow> R,G \<turnstile>\<^sub>w M \<ge> P \<Longrightarrow> R,G \<turnstile>\<^sub>w M {c} Q"
+  by (auto simp: valid_def context_order_def)
+
+text \<open>Assert Rule\<close>
+lemma assert_wp:
+  assumes "A \<Longrightarrow> R,G \<turnstile>\<^sub>w P {c} Q"
+  shows "R,G \<turnstile>\<^sub>w (P \<inter> assert A) {c} Q"
+proof (cases A)
+  case True
+  then show ?thesis using assms by (intro rewrite_wp[OF _ assert_ord], simp)
+next
+  case False
+  then show ?thesis by (intro false_wp, auto simp: assert_def)
+qed 
+
+text \<open>Com Rule\<close>
+theorem com_wp:
+  shows "R,G \<turnstile>\<^sub>w wp R c Q {c} Q" 
+proof (induct c arbitrary: Q)
+  case Skip
+  then show ?case by (auto simp: valid_def)
+next
+  case (Op x1 x2)
+  then show ?case unfolding valid_def lift\<^sub>c.simps 
+    by (intro conjI impI basic_wp\<^sub>i_1) auto
+next
+  case (Seq c1 c2)
+  then show ?case by (auto simp: valid_def)
+next
+  case (If x1 c1 c2)
+  then show ?case unfolding wp.simps by (blast intro: if_wp)
+next
+  case (While x1 x2 c)
+  then show ?case unfolding wp.simps by (intro assert_wp impI while_wp) (auto)
+next
+  case (DoWhile I c b)
+  thus ?case unfolding wp.simps by (intro assert_wp do_wp; rule rewrite_wp) auto
+qed
+
+subsection \<open>High-Level Theorem\<close>
+
+text \<open>Soundness lemma for WP reasoning\<close>
+theorem armv8_wp_sound:
+  assumes wf: "transitive R" "reflexive R" "reflexive G" 
+  assumes st: "stable\<^sub>t R Q" 
+  assumes g: "guar\<^sub>c c G"
+  assumes P: "P \<subseteq> wp R c Q"
+  shows "\<Turnstile> c SAT [P, R, G, Q]"
+proof -
+  have "R,G \<turnstile>\<^sub>s wp R c Q {c} Q" using wf st g com_wp unfolding valid_def by blast
+  hence "R,G \<turnstile>\<^sub>s P {c} Q" by (rule rules.conseq) (insert P, auto simp: )
+  thus ?thesis by (intro sound thread) auto
+qed
 
 end
