Peterson.thy
@@ -1,0 +1,66 @@
+theory Peterson
+  imports SimAsm_Syntax
+begin
+
+datatype globals = flag0 | flag1 | turn
+record aux = 
+  a0 :: bool 
+  a1 :: bool
+
+lemma peterson0:
+  "FNBEGIN
+    R: \<^sup>1\<lbrakk>flag0\<rbrakk> = \<^sup>2\<lbrakk>flag0\<rbrakk> \<and> (\<^sup>1\<lbrakk>turn\<rbrakk> \<longrightarrow> \<^sup>2\<lbrakk>turn\<rbrakk>)
+    G: \<^sup>1\<lbrakk>flag1\<rbrakk> = \<^sup>2\<lbrakk>flag1\<rbrakk> \<and> (\<^sup>1\<lbrakk>turn\<rbrakk> \<longrightarrow> \<^sup>2\<lbrakk>turn\<rbrakk>)
+    P: True
+    {
+      \<lbrakk>flag0\<rbrakk> := #True;
+      fence;
+      \<lbrakk>turn\<rbrakk> := #True;
+      fence;
+      do
+        \<^bold>r0 := \<lbrakk>flag1\<rbrakk>, \<^sup>aa0 := \<^sup>0\<lbrakk>flag1\<rbrakk>;
+        \<^bold>r1 := \<lbrakk>turn\<rbrakk>
+      while (\<^bold>r0 && \<^bold>r1);
+      Skip;
+      \<lbrakk>flag0\<rbrakk> := #False
+    }
+    Q: True
+  FNEND" 
+  apply(unfold fn_valid.simps, intro conjI)
+
+  apply (auto simp: step\<^sub>t_def stable_def reflexive_def transitive_def)[4]
+
+  apply (clarsimp simp: aux_upd_def step_def glb_def wp\<^sub>r_def)
+
+  sorry
+
+
+lemma peterson1:
+  "FNBEGIN
+    R: True
+    G: \<^sup>1\<lbrakk>flag0\<rbrakk> = \<^sup>2\<lbrakk>flag0\<rbrakk> \<and> (\<^sup>1\<lbrakk>turn\<rbrakk> = 0 \<longrightarrow> \<^sup>2\<lbrakk>turn\<rbrakk> = 0)
+    P: True
+    {
+      \<lbrakk>flag1\<rbrakk> := true;
+      \<lbrakk>turn\<rbrakk> := #0;
+      while (\<lbrakk>flag0\<rbrakk> == true) && (\<lbrakk>turn\<rbrakk> == #0)
+      do
+        Skip
+      od;
+      \<^bold>r0 := \<^bold>r2;
+      \<lbrakk>flag1\<rbrakk> := false
+    }
+    Q: True
+  FNEND" 
+  apply(unfold fn_valid.simps, intro conjI)
+
+  apply (auto simp: step\<^sub>t_def stable_def reflexive_def transitive_def)[4]
+
+  apply (clarsimp simp: step_def glb_def wp\<^sub>r_def)
+
+  apply (simp add: stabilize_def assert_def)
+
+  done
+
+
+end
