StoreBuffer.thy
@@ -1,0 +1,51 @@
+theory StoreBuffer
+  imports SimAsm_Syntax
+begin
+
+datatype globals = X | Y
+record aux = S :: nat 
+
+lemma sb0:
+  "FNBEGIN
+    R: (\<^sup>1\<^sup>aS \<in> {1,2} \<longrightarrow> \<^sup>2\<^sup>aS \<in> {1,2}) \<and> (\<^sup>1\<^sup>aS = 2 \<longrightarrow> \<^sup>2\<^sup>aS = 2)
+    G: (\<^sup>1\<^sup>aS \<in> {1,2} \<longrightarrow> \<^sup>2\<^sup>aS \<in> {1,2}) \<and> (\<^sup>1\<^sup>aS = 1 \<longrightarrow> \<^sup>2\<^sup>aS = 1)
+    P: True
+    {
+      \<lbrakk>X\<rbrakk> := #1;
+      fence;
+      \<^bold>r0 := \<lbrakk>Y\<rbrakk> :\<^sub>a \<^sup>aS := (if \<^sup>aS = 0 then 1 else \<^sup>aS)
+    }
+    Q: (\<^sup>aS \<in> {1,2} \<and> (\<^sup>aS = 2 \<longrightarrow> \<^sup>0\<^bold>r0 = 1))
+  FNEND" 
+  unfolding fn_valid.simps
+  apply (intro conjI)
+
+  defer 1
+
+  apply (auto simp: reflexive_def transitive_def)[3]
+
+  apply (auto simp: wp\<^sub>r_def st_upd_def step_def glb_def aux_upd_def)[1]
+  
+  apply (clarsimp simp: stabilize_def wp\<^sub>r_def st_upd_def step_def glb_def aux_upd_def)[1]
+
+  sorry
+
+  apply (auto simp: glb_def step\<^sub>t_def stable_def)[1]
+
+  sorry
+
+lemma sb1:
+  "FNBEGIN
+    R: True
+    G: True
+    P: True
+    {
+      \<lbrakk>Y\<rbrakk> := #1;
+      fence;
+      \<^bold>r1 := \<lbrakk>X\<rbrakk>
+    }
+    Q: (\<^sup>0\<^bold>r0 = 1 \<or> \<^sup>0\<^bold>r1 = 1)
+  FNEND" 
+  sorry
+
+end
